prove modified end to end helper lemma that has weaker assumptions
1) don't require the initial state relation to map every constant to itself
2) don't require constants to be shared between locals and globals

BoogieLang/PassificationEndToEnd.thy
@@ -8,22 +8,43 @@ fun initial_set :: "'a absval_ty_fun \<Rightarrow> passive_rel \<Rightarrow> var
               (\<forall>x y. R x = Some (Inl y) \<longrightarrow> lookup_var \<Lambda> ns x = lookup_var \<Lambda>' u y) \<and>
               binder_state u = Map.empty}"
 
-fun initial_state :: "'a absval_ty_fun \<Rightarrow> rtype_env \<Rightarrow> passive_rel \<Rightarrow> var_context \<Rightarrow> var_context \<Rightarrow> 'a nstate \<Rightarrow> 'a named_state"
-  where "initial_state A \<Omega> R \<Lambda> \<Lambda>' ns x = 
-         (if (\<exists>z. R z = Some (Inl x)) then 
-            lookup_var \<Lambda> ns (SOME z. R z = Some (Inl x)) 
-          else 
-            (case (map_of (snd \<Lambda>') x) of Some \<tau> \<Rightarrow> Some (val_of_type A (instantiate \<Omega> \<tau>)) | None \<Rightarrow> None)             
-         )"
+fun initial_state_local :: "'a absval_ty_fun \<Rightarrow> rtype_env \<Rightarrow> passive_rel \<Rightarrow> var_context \<Rightarrow> var_context \<Rightarrow> 'a nstate \<Rightarrow> 'a named_state"
+  where "initial_state_local A \<Omega> R \<Lambda> \<Lambda>' ns x = 
+         (case (map_of (snd \<Lambda>') x) of Some \<tau> =>
+           (if (\<exists>z. R z = Some (Inl x)) then 
+              lookup_var \<Lambda> ns (SOME z. R z = Some (Inl x)) 
+            else 
+              ( Some (val_of_type A (instantiate \<Omega> \<tau>)))             
+           )
+          | None \<Rightarrow> None)"
+
+fun initial_state_global :: "'a absval_ty_fun \<Rightarrow> rtype_env \<Rightarrow> passive_rel \<Rightarrow> var_context \<Rightarrow> var_context \<Rightarrow> 'a nstate \<Rightarrow> 'a named_state"
+  where "initial_state_global A \<Omega> R \<Lambda> \<Lambda>' ns x = 
+           (case (map_of (fst \<Lambda>') x) of Some \<tau> =>
+           (if (\<exists>z. R z = Some (Inl x)) then 
+              lookup_var \<Lambda> ns (SOME z. R z = Some (Inl x)) 
+            else 
+              ( Some (val_of_type A (instantiate \<Omega> \<tau>)))             
+           )
+          | None \<Rightarrow> None)"
 
 definition rel_range
   where "rel_range R = {y. \<exists>x. R x = Some (Inl y)}"
 
-lemma initial_state_lookup:
-  assumes "inj R" and "R x = Some (Inl y)"
-  shows "initial_state A \<Omega> R \<Lambda> \<Lambda>' ns y = lookup_var \<Lambda> ns x" (is "?u y = lookup_var \<Lambda> ns x")
+lemma initial_state_lookup: 
+  assumes "inj R" and "R x = Some (Inl y)" and "map_of (snd \<Lambda>') y = Some vd"
+  shows "initial_state_local A \<Omega> R \<Lambda> \<Lambda>' ns y = lookup_var \<Lambda> ns x" (is "?u y = lookup_var \<Lambda> ns x")
 proof -
-  from \<open>R x = Some (Inl y)\<close> have "?u y = (lookup_var \<Lambda> ns (SOME z. R z = Some (Inl y)))" by auto
+  from \<open>R x = Some (Inl y)\<close> \<open>map_of (snd \<Lambda>') y = Some vd\<close> have "?u y = (lookup_var \<Lambda> ns (SOME z. R z = Some (Inl y)))" by auto
+  thus "?u y = lookup_var \<Lambda> ns x" using \<open>inj R\<close>
+    by (metis assms(2) inv_def inv_f_f) 
+qed
+
+lemma initial_state_global_lookup: 
+  assumes "inj R" and "R x = Some (Inl y)" and "map_of (fst \<Lambda>') y = Some vd"
+  shows "initial_state_global A \<Omega> R \<Lambda> \<Lambda>' ns y = lookup_var \<Lambda> ns x" (is "?u y = lookup_var \<Lambda> ns x")
+proof -
+  from \<open>R x = Some (Inl y)\<close> \<open>map_of (fst \<Lambda>') y = Some vd\<close> have "?u y = (lookup_var \<Lambda> ns (SOME z. R z = Some (Inl y)))" by auto
   thus "?u y = lookup_var \<Lambda> ns x" using \<open>inj R\<close>
     by (metis assms(2) inv_def inv_f_f) 
 qed
@@ -34,29 +55,28 @@ lemma init_state_elem_init_set:
           Closed:"\<And>y \<tau>. \<not>(\<exists> x. R x = Some (Inl y)) \<Longrightarrow> lookup_var_ty \<Lambda>' y = Some \<tau> \<Longrightarrow> closed (instantiate \<Omega> \<tau>)" and          
           RelTy:"\<And>x y. R x = Some (Inl y) \<Longrightarrow> lookup_var_ty \<Lambda> x = lookup_var_ty \<Lambda>' y" and
           RelWt:"rel_well_typed A \<Lambda> \<Omega> R ns" and
-          Consts:"fst \<Lambda> = (fst \<Lambda>')@globals" and
-          R_consts:"list_all (\<lambda>vd. R (fst vd) = Some (Inl (fst vd))) (fst \<Lambda>')" and
                 "inj R" and
        (* no shadowing *)
           ConstsDisj:"set (map fst (fst \<Lambda>')) \<inter> set (map fst (snd \<Lambda>)) = {}" and
           ConstsDisj2:"set (map fst (fst \<Lambda>')) \<inter> set (map fst (snd \<Lambda>')) = {}"
         shows "\<lparr>old_global_state = Map.empty, 
-               global_state = global_state ns, 
-               local_state = (initial_state A \<Omega> R \<Lambda> \<Lambda>' ns), 
+               global_state = (initial_state_global A \<Omega> R \<Lambda> \<Lambda>' ns), 
+               local_state = (initial_state_local A \<Omega> R \<Lambda> \<Lambda>' ns), 
                binder_state = Map.empty \<rparr> \<in> initial_set A R \<Lambda> \<Lambda>' \<Omega> ns" (is "?u \<in> ?U")
 proof (simp only: initial_set.simps, rule, intro conjI)
   show "state_typ_wf A \<Omega> (local_state ?u) (snd \<Lambda>')"
     unfolding state_typ_wf_def
   proof ((rule allI)+, rule impI)
     fix y \<tau>
-    assume "map_of (snd \<Lambda>') y = Some \<tau>"
+    assume localy:"map_of (snd \<Lambda>') y = Some \<tau>"
     hence LookupTyY:"lookup_var_ty \<Lambda>' y = Some \<tau>"
       by (simp add: lookup_var_ty_local) 
     show "map_option (type_of_val A) (local_state ?u y) = Some (instantiate \<Omega> \<tau>)"
     proof (cases "\<exists>x. R x = Some (Inl y)")
       case True
       from this obtain x where "R x = Some (Inl y)" by auto
-      hence LookupUY:"local_state ?u y = lookup_var \<Lambda> ns x" using initial_state_lookup[OF \<open>inj R\<close>] by fastforce
+      hence LookupUY:"local_state ?u y = lookup_var \<Lambda> ns x"
+          by (metis (no_types) \<open>R x = Some (Inl y)\<close> initial_state_lookup[OF \<open>inj R\<close>] localy nstate.select_convs(3))
       from RelTy RelWt obtain v where
               "lookup_var \<Lambda> ns x = Some v" and "type_of_val A v = instantiate \<Omega> \<tau>"
         unfolding rel_well_typed_def using LookupTyY \<open>R x = Some (Inl y)\<close>
@@ -75,27 +95,31 @@ next
     unfolding state_typ_wf_def
   proof ((rule allI)+, rule impI)
     fix y \<tau>
-    assume "map_of (fst \<Lambda>') y = Some \<tau>"
+    assume global_y:"map_of (fst \<Lambda>') y = Some \<tau>"
     from this moreover have "map_of (snd \<Lambda>') y = None" using ConstsDisj2
       by (metis disjoint_iff_not_equal list.set_map map_of_eq_None_iff option.distinct(1)) 
     ultimately have LookupTyY:"lookup_var_ty \<Lambda>' y = Some \<tau>"
       by (simp add: lookup_var_ty_global) 
     from \<open>map_of (fst \<Lambda>') y = Some \<tau>\<close> have "(y, \<tau>) \<in> set (fst \<Lambda>')" 
       by (simp add: map_of_SomeD) 
-    hence "R y = Some (Inl y)" using R_consts using split_list by fastforce
-    hence "lookup_var_ty \<Lambda> y = Some \<tau>" using LookupTyY RelTy by simp
-    with RelTy RelWt obtain v where
-              Aux1:"lookup_var \<Lambda> ns y = Some v" and Aux2:"type_of_val A v = instantiate \<Omega> \<tau>"
-        unfolding rel_well_typed_def using LookupTyY \<open>R y = Some (Inl y)\<close> by force 
-    from \<open>map_of (fst \<Lambda>') y = Some \<tau>\<close> \<open>map_of (snd \<Lambda>') y = None\<close>
-    have "lookup_var \<Lambda>' ?u y = global_state ?u y" 
-      by (metis lookup_var_global prod.collapse)
-    moreover from \<open>map_of (fst \<Lambda>') y = Some \<tau>\<close> \<open>map_of (snd \<Lambda>') y = None\<close> have
-       "lookup_var \<Lambda> ns y = global_state ns y" using Consts ConstsDisj2
-      by (metis ConstsDisj disjoint_iff_not_equal image_set lookup_var_global map_of_eq_None_iff option.distinct(1) surjective_pairing)     
-    ultimately show
-      "map_option (type_of_val A) (global_state ?u y) =  Some (instantiate \<Omega> \<tau>)" using Aux1 Aux2
-      by force     
+    show "map_option (type_of_val A) (global_state ?u y) = Some (instantiate \<Omega> \<tau>)"
+    proof (cases "\<exists>x. R x = Some (Inl y)")
+      case True
+      from this obtain x where "R x = Some (Inl y)" by auto
+      hence LookupUY:"global_state ?u y = lookup_var \<Lambda> ns x"
+        by (metis \<open>R x = Some (Inl y)\<close> initial_state_global_lookup[OF \<open>inj R\<close>] global_y nstate.select_convs(2))
+      from RelTy RelWt obtain v where
+              "lookup_var \<Lambda> ns x = Some v" and "type_of_val A v = instantiate \<Omega> \<tau>"
+        unfolding rel_well_typed_def using LookupTyY \<open>R x = Some (Inl y)\<close>
+        by fastforce 
+      thus ?thesis using LookupUY by auto
+    next
+      case False
+      hence "global_state ?u y = Some (val_of_type A (instantiate \<Omega> \<tau>))"
+        by (simp add: global_y) 
+      thus ?thesis using  False LookupTyY Closed val_of_type_correct NonEmptyTypes
+        by blast      
+    qed
   qed
 next
   show "\<forall> x y. R x = Some (Inl y) \<longrightarrow> lookup_var \<Lambda> ns x = lookup_var \<Lambda>' ?u y"
@@ -104,30 +128,26 @@ next
     assume "R x = Some (Inl y)"
     hence SameTy:"lookup_var_ty \<Lambda> x = lookup_var_ty \<Lambda>' y" using RelTy by simp
     moreover from \<open>R x = Some (Inl y)\<close> RelWt obtain \<tau> where LookupX:"lookup_var_ty \<Lambda> x = Some \<tau>"
-      by (meson rel_well_typed_def)    
+      by (meson rel_well_typed_def)
+    hence "lookup_var_ty \<Lambda>' y = Some \<tau>" using RelTy[OF \<open>R x = Some (Inl y)\<close>] by simp    
     show "lookup_var \<Lambda> ns x = lookup_var \<Lambda>' ?u y"
     proof (cases "map_of (snd \<Lambda>') y = None")
       case True
-      with SameTy LookupX have "map_of (fst \<Lambda>') y = Some \<tau>"
-        by (simp add: lookup_var_ty_def) 
-      hence "(y,\<tau>) \<in> set (fst \<Lambda>')"
-        by (simp add: map_of_SomeD) 
-      with R_consts have "R y = Some (Inl y)" using split_list by fastforce 
-      with  \<open>inj R\<close> \<open>R x = Some (Inl y)\<close> have "x = y" using inj_eq by fastforce   
-      from \<open>map_of (fst \<Lambda>') y = Some \<tau>\<close> have "map_of (fst \<Lambda>) y = Some \<tau>" using Consts by simp
-      moreover with ConstsDisj have "map_of (snd \<Lambda>) y = None"
-        by (metis \<open>map_of (fst \<Lambda>') y = Some \<tau>\<close> disjoint_iff_not_equal image_set map_of_eq_None_iff option.distinct(1)) 
-      ultimately have "lookup_var \<Lambda> ns x = global_state ns x" using \<open>x = y\<close>
-        by (metis lookup_var_global prod.exhaust_sel) 
-      then show ?thesis using \<open>x = y\<close> \<open>map_of (snd \<Lambda>') y = None\<close> \<open>map_of (fst \<Lambda>') y = Some \<tau>\<close>
-        by (metis lookup_var_global nstate.select_convs(2) surjective_pairing) 
+      hence global_y:"map_of (fst \<Lambda>') y = Some \<tau>" using \<open>lookup_var_ty \<Lambda>' y = Some \<tau>\<close> 
+        by (simp add: lookup_var_ty_global_3)
+      from True have "lookup_var \<Lambda>' ?u y = global_state ?u y"
+        by (simp add: lookup_var_def)
+      hence "\<dots> = (lookup_var \<Lambda> ns (SOME z. R z = Some (Inl y)))" using \<open>R x = Some (Inl y)\<close> True  global_y
+        by auto
+      then show ?thesis using \<open>inj R\<close> \<open>R x = Some (Inl y)\<close> 
+        by (metis \<open>lookup_var \<Lambda>' ?u y = global_state ?u y\<close> global_y initial_state_global_lookup nstate.select_convs(2))
     next
       case False
       hence "lookup_var \<Lambda>' ?u y = local_state ?u y"
-        by (metis lookup_var_local option.exhaust_sel prod.collapse snd_def)      
-      hence "\<dots> = (lookup_var \<Lambda> ns (SOME z. R z = Some (Inl y)))" using \<open>R x = Some (Inl y)\<close> by auto      
+        by (metis lookup_var_local option.exhaust_sel prod.collapse)      
+      hence "\<dots> = (lookup_var \<Lambda> ns (SOME z. R z = Some (Inl y)))" using \<open>R x = Some (Inl y)\<close> False by auto      
       then show ?thesis using \<open>inj R\<close> \<open>R x = Some (Inl y)\<close> initial_state_lookup
-        by (metis \<open>lookup_var \<Lambda>' \<lparr>old_global_state = Map.empty, global_state = global_state ns, local_state = initial_state A \<Omega> R \<Lambda> \<Lambda>' ns, binder_state = Map.empty\<rparr> y = local_state \<lparr>old_global_state = Map.empty, global_state = global_state ns, local_state = initial_state A \<Omega> R \<Lambda> \<Lambda>' ns, binder_state = Map.empty\<rparr> y\<close> nstate.select_convs(3))
+        by (metis False \<open>lookup_var \<Lambda>' ?u y = local_state ?u y\<close> nstate.select_convs(3) option.collapse)
     qed
   qed
 next
@@ -288,5 +308,14 @@ lemma rel_well_typed_state_typ_wf:
   using RelWtConst
 
   using \<open>\<And>x \<tau>. lookup_var_ty \<Lambda> x = Some \<tau> \<Longrightarrow> \<exists>v. lookup_var \<Lambda> ns x = Some v \<and> type_of_val A v = instantiate \<Omega> \<tau>\<close> by force
+
+lemma rel_well_typed_state_typ_wf_2: 
+  assumes RelWtVar:"\<And>x y. R x = Some z \<Longrightarrow> \<exists>\<tau> y. z = Inl y \<and> lookup_var_ty \<Lambda> x = Some \<tau>" and          
+          S1:"state_typ_wf A \<Omega> (local_state ns) (snd \<Lambda>)" and
+          S2:"state_typ_wf A \<Omega> (global_state ns) (fst \<Lambda>)"
+        shows "rel_well_typed A \<Lambda> \<Omega> R ns"
+  using assms rel_well_typed_state_typ_wf[OF _ _ S1 S2]
+  oops
+
 
 end
